src/opt/ReorderLoad.v
@@ -58,33 +58,85 @@ Inductive reorder_load r1 l1 o1: forall (i2:Instr.t), Prop :=
     reorder_load r1 l1 o1 (Instr.fence or2 ow2)
 .
 
-Inductive sim_load: forall (st_src:lang.(Language.state)) (lc_src:Local.t) (sc_k_src:TimeMap.t) (mem_k_src:Memory.t)
-                      (st_tgt:lang.(Language.state)) (lc_tgt:Local.t) (sc_k_tgt:TimeMap.t) (mem_k_tgt:Memory.t), Prop :=
+Inductive sim_load: forall (st_src:lang.(Language.state)) (lc_src:Local.t) (sc0_src:TimeMap.t) (mem0_src:Memory.t)
+                      (st_tgt:lang.(Language.state)) (lc_tgt:Local.t) (sc0_tgt:TimeMap.t) (mem0_tgt:Memory.t), Prop :=
 | sim_load_intro
     r1 l1 ts1 v1 released1 o1 i2
     rs lc1_src lc1_tgt lc2_src
-    sc_k_src sc_k_tgt
-    mem_k_src mem_k_tgt
+    sc0_src sc0_tgt
+    mem0_src mem0_tgt
     (REORDER: reorder_load r1 l1 o1 i2)
-    (READ: Local.read_step lc1_src mem_k_src l1 ts1 v1 released1 o1 lc2_src)
+    (READ: Local.read_step lc1_src mem0_src l1 ts1 v1 released1 o1 lc2_src)
+    (WF_SRC: Local.wf lc1_src mem0_src)
+    (WF_TGT: Local.wf lc1_tgt mem0_tgt)
+    (SC_SRC: Memory.closed_timemap sc0_src mem0_src)
+    (SC_TGT: Memory.closed_timemap sc0_tgt mem0_tgt)
+    (CLOSED_SRC: Memory.closed mem0_src)
+    (CLOSED_TGT: Memory.closed mem0_tgt)
     (LOCAL: sim_local lc2_src lc1_tgt):
     sim_load
-      (State.mk rs [Stmt.instr i2; Stmt.instr (Instr.load r1 l1 o1)]) lc1_src sc_k_src mem_k_src
-      (State.mk (RegFun.add r1 v1 rs) [Stmt.instr i2]) lc1_tgt sc_k_tgt mem_k_tgt
+      (State.mk rs [Stmt.instr i2; Stmt.instr (Instr.load r1 l1 o1)]) lc1_src sc0_src mem0_src
+      (State.mk (RegFun.add r1 v1 rs) [Stmt.instr i2]) lc1_tgt sc0_tgt mem0_tgt
 .
 
+Lemma sim_load_future
+      st_src lc_src sc1_src mem1_src
+      st_tgt lc_tgt sc1_tgt mem1_tgt
+      sc2_src mem2_src
+      (SC1: TimeMap.le sc1_src sc1_tgt)
+      (MEM1: Memory.sim mem1_tgt mem1_src)
+      (SIM1: sim_load st_src lc_src sc1_src mem1_src
+                      st_tgt lc_tgt sc1_tgt mem1_tgt)
+      (SC_FUTURE_SRC: TimeMap.le sc1_src sc2_src)
+      (MEM_FUTURE_SRC: Memory.future mem1_src mem2_src)
+      (WF_SRC: Local.wf lc_src mem2_src)
+      (SC_SRC: Memory.closed_timemap sc2_src mem2_src)
+      (MEM_SRC: Memory.closed mem2_src):
+  exists lc'_src sc2_tgt mem2_tgt,
+    <<SC2: TimeMap.le sc2_src sc2_tgt>> /\
+    <<MEM2: Memory.sim mem2_tgt mem2_src>> /\
+    <<SC_FUTURE_TGT: TimeMap.le sc1_tgt sc2_tgt>> /\
+    <<MEM_FUTURE_TGT: Memory.future mem1_tgt mem2_tgt>> /\
+    <<WF_TGT: Local.wf lc_tgt mem2_tgt>> /\
+    <<SC_TGT: Memory.closed_timemap sc2_tgt mem2_tgt>> /\
+    <<MEM_TGT: Memory.closed mem2_tgt>> /\
+    <<SIM2: sim_load st_src lc'_src sc2_src mem2_src
+                     st_tgt lc_tgt sc2_tgt mem2_tgt>>.
+Proof.
+  inv SIM1.
+  exploit future_read_step; try apply READ; eauto. i. des.
+  exploit sim_local_future; try apply MEM1; eauto.
+  { inv LOCAL. apply MemInv.sem_bot_inv in PROMISES; auto. rewrite <- PROMISES.
+    inv READ. ss. apply MemInv.sem_bot.
+  }
+  { inv LOCAL. rewrite PROMISES_LE.
+    inv READ. ss.
+  }
+  i. des. esplits; eauto.
+  - etrans.
+    + apply Memory.max_timemap_spec; eauto. committac.
+    + apply Memory.sim_max_timemap; eauto.
+  - etrans.
+    + apply Memory.max_timemap_spec; eauto. committac.
+    + apply Memory.future_max_timemap; eauto.
+  - apply Memory.max_timemap_closed. committac.
+  - econs; eauto.
+    + apply Memory.max_timemap_closed. committac.
+    + etrans; eauto.
+Qed.
+
 Lemma sim_load_step
-      st1_src lc1_src sc_k_src mem_k_src
-      st1_tgt lc1_tgt sc_k_tgt mem_k_tgt
-      (SIM: sim_load st1_src lc1_src sc_k_src mem_k_src
-                     st1_tgt lc1_tgt sc_k_tgt mem_k_tgt):
+      st1_src lc1_src sc0_src mem0_src
+      st1_tgt lc1_tgt sc0_tgt mem0_tgt
+      (SIM: sim_load st1_src lc1_src sc0_src mem0_src
+                     st1_tgt lc1_tgt sc0_tgt mem0_tgt):
   forall sc1_src sc1_tgt mem1_src mem1_tgt
     (SC: TimeMap.le sc1_src sc1_tgt)
     (MEMORY: Memory.sim mem1_tgt mem1_src)
-    (SC_FUTURE_SRC: TimeMap.le sc_k_src sc1_src)
-    (SC_FUTURE_TGT: TimeMap.le sc_k_tgt sc1_tgt)
-    (MEM_FUTURE_SRC: Memory.future mem_k_src mem1_src)
-    (MEM_FUTURE_TGT: Memory.future mem_k_tgt mem1_tgt)
+    (SC_FUTURE_SRC: TimeMap.le sc0_src sc1_src)
+    (SC_FUTURE_TGT: TimeMap.le sc0_tgt sc1_tgt)
+    (MEM_FUTURE_SRC: Memory.future mem0_src mem1_src)
+    (MEM_FUTURE_TGT: Memory.future mem0_tgt mem1_tgt)
     (WF_SRC: Local.wf lc1_src mem1_src)
     (WF_TGT: Local.wf lc1_tgt mem1_tgt)
     (SC_SRC: Memory.closed_timemap sc1_src mem1_src)
@@ -95,6 +147,7 @@ Lemma sim_load_step
                      st1_src lc1_src sc1_src mem1_src
                      st1_tgt lc1_tgt sc1_tgt mem1_tgt.
 Proof.
+  ii. exploit sim_load_future; try apply SIM; eauto.
   inv SIM. ii.
   exploit future_read_step; try apply READ; eauto. i. des.
   inv STEP_TGT; inv STEP0; try (inv STATE; inv INSTR; inv REORDER); ss.
@@ -103,12 +156,13 @@ Proof.
     { eapply Local.read_step_future; eauto. }
     i. des.
     exploit reorder_read_promise; try apply x0; try apply STEP_SRC; eauto. i. des.
+    exploit Local.promise_step_future; eauto. i. des.
     esplits; try apply SC; eauto.
-    + econs. econs. eauto.
+    + econs 2. econs. econs. eauto.
     + eauto.
     + right. econs; eauto. etrans; eauto.
   - (* load *)
-    exploit sim_local_read; (try by etrans; eauto); eauto.
+    exploit sim_local_read; (try by etrans; eauto); eauto; try refl.
     { eapply Local.read_step_future; eauto. }
     i. des.
     exploit reorder_read_read; try apply STEP; try apply STEP_SRC; eauto. i. des.
@@ -116,7 +170,7 @@ Proof.
     + econs 2; [|econs 1]. econs.
       * econs 2. econs 2; eauto. econs. econs.
       * eauto.
-    + econs 2. econs 2; eauto. econs. econs.
+    + econs 2. econs 2. econs 2; eauto. econs. econs.
     + eauto.
     + eauto.
     + eauto.
@@ -139,24 +193,24 @@ Proof.
         { econs. }
         { apply RegFile.eq_except_singleton. }
       * eauto.
-    + econs 2. econs 2; eauto. econs. econs.
+    + econs 2. econs 2. econs 2; eauto. econs. econs.
     + eauto.
     + eauto.
-    + eauto.
+    + etrans; eauto.
     + left. eapply paco9_mon; [apply sim_stmts_nil|]; ss. etrans; eauto.
   - (* update *)
-    exploit sim_local_read; (try by etrans; eauto); eauto.
+    exploit sim_local_read; (try by etrans; eauto); eauto; try refl.
     { eapply Local.read_step_future; eauto. }
     i. des.
+    exploit reorder_read_read; try apply STEP; try apply STEP_SRC; eauto. i. des.
     exploit sim_local_write; try apply SC; try apply LOCAL1; (try by etrans; eauto); eauto.
-    { admit. }
+    { inv LOCAL1. eapply MEM_TGT; eauto. }
     { eapply Local.read_step_future; eauto.
       eapply Local.read_step_future; eauto.
     }
     { eapply Local.read_step_future; eauto. }
     i. des.
-    exploit reorder_read_read; try apply STEP; try apply STEP_SRC; eauto. i. des.
-    exploit reorder_read_write; try apply STEP2; try apply LOCAL2; eauto.
+    exploit reorder_read_write; try apply STEP_SRC0; try apply STEP2; eauto.
     { eapply Local.read_step_future; eauto. }
     i. des.
     esplits.
@@ -167,15 +221,17 @@ Proof.
         apply RegSet.singleton_spec in LHS. subst.
         apply RegSet.add_spec. auto.
       * eauto.
-    + econs 2. econs 2; eauto. econs. econs.
+    + econs 2. econs 2. econs 2; eauto. econs. econs.
     + eauto.
     + eauto.
+    + etrans; eauto.
     + left. eapply paco9_mon; [apply sim_stmts_nil|]; ss.
-      apply RegFun.add_add. ii. subst. eapply REGS.
-      * apply RegSet.singleton_spec. eauto.
-      * apply RegSet.add_spec. eauto.
+      * apply RegFun.add_add. ii. subst. eapply REGS.
+        { apply RegSet.singleton_spec. eauto. }
+        { apply RegSet.add_spec. eauto. }
+      * etrans; eauto.
   - (* fence *)
-    exploit sim_local_fence; eauto.
+    exploit sim_local_fence; try apply SC; try apply LOCAL1; (try by etrans; eauto); eauto; try refl.
     { eapply Local.read_step_future; eauto. }
     i. des.
     exploit reorder_read_fence; try apply x0; try apply STEP_SRC; eauto. i. des.
@@ -183,18 +239,44 @@ Proof.
     + econs 2; [|econs 1]. econs.
       * econs 2. econs 5; eauto. econs. econs.
       * eauto.
-    + econs 2. econs 2; eauto. econs. econs.
+    + econs 2. econs 2. econs 2; eauto. econs. econs.
     + eauto.
+    + etrans; eauto.
     + eauto.
     + left. eapply paco9_mon; [apply sim_stmts_nil|]; ss.
+      etrans; eauto.
 Qed.
 
 Lemma sim_load_sim_thread:
-  sim_load <6= (sim_thread (sim_terminal eq)).
+  sim_load <8= (sim_thread (sim_terminal eq)).
 Proof.
   pcofix CIH. i. pfold. ii. ss. splits; ss.
   - i. inv TERMINAL_TGT. inv PR; ss.
-  - i. inv PR. eapply sim_local_future; try apply LOCAL; eauto.
+  - i. inv PR.
+    exploit future_read_step; try apply MEM_FUTURE_SRC; eauto. i. des.
+    rewrite LOCAL in LOCAL0.
+    exploit sim_local_future; try apply LOCAL0; eauto.
+    { eapply Local.read_step_future; eauto. }
+    { exploit future_read_step; try apply STEP; eauto. i. des.
+      exploit Local.read_step_future; eauto. i. des.
+      
+  }
+    
+    exploit Local.read_step_future; eauto. i. des.
+    exploit sim_local_future; try apply LOCAL0; try apply x0; eauto.
+    { 
+    etrans. eauto. eauto.
+    ; (try by etrans; eauto); eauto. try apply STEP; eauto.
+      esplits; eauto.
+      - etrans.
+        + apply Memory.max_timemap_spec; eauto. committac.
+        + apply Memory.sim_max_timemap; eauto.
+      - etrans.
+        + apply Memory.max_timemap_spec; eauto. committac.
+        + apply Memory.future_max_timemap; eauto.
+      - apply Memory.max_timemap_closed. committac.
+    }
+    exploit sim_local_future; try apply LOCAL; eauto.
     + eapply Local.read_step_future; eauto.
       eapply Local.future_read_step; eauto.
     + eapply Local.read_step_future; eauto.
