src/opt/ReorderUpdate.v
@@ -57,31 +57,31 @@ Inductive reorder_update r1 l1 rmw1 or1 ow1: forall (i2:Instr.t), Prop :=
     reorder_update r1 l1 rmw1 or1 ow1 (Instr.update r2 l2 rmw2 or2 ow2)
 .
 
-Inductive sim_update: forall (st_src:lang.(Language.state)) (lc_src:Local.t) (sc_k_src:TimeMap.t) (mem_k_src:Memory.t)
-                        (st_tgt:lang.(Language.state)) (lc_tgt:Local.t) (sc_k_tgt:TimeMap.t) (mem_k_tgt:Memory.t), Prop :=
+Inductive sim_update: forall (st_src:lang.(Language.state)) (lc_src:Local.t) (sc0_src:TimeMap.t) (mem0_src:Memory.t)
+                        (st_tgt:lang.(Language.state)) (lc_tgt:Local.t) (sc0_tgt:TimeMap.t) (mem0_tgt:Memory.t), Prop :=
 | sim_update_intro
     r1 l1 from1 to1 vr1 vret1 vw1 releasedr1 releasedw1 rmw1 or1 ow1 i2
     rs lc1_src lc1_tgt lc2_src lc3_src
-    mem_k_src mem_k_tgt
+    mem0_src mem0_tgt
     (REORDER: reorder_update r1 l1 rmw1 or1 ow1 i2)
     (RMW: RegFile.eval_rmw rs rmw1 vr1 = (vret1, vw1))
-    (READ: Local.read_step lc1_src sc_k_src mem_k_src l1 from1 vr1 releasedr1 or1 lc2_src)
-    (FULFILL: Local.fulfill_step lc2_src mem_k_src l1 from1 to1 vw1 releasedw1 (Capability.join releasedr1 releasedw1) ow1 lc3_src)
+    (READ: Local.read_step lc1_src sc0_src mem0_src l1 from1 vr1 releasedr1 or1 lc2_src)
+    (FULFILL: Local.fulfill_step lc2_src mem0_src l1 from1 to1 vw1 releasedw1 (Capability.join releasedr1 releasedw1) ow1 lc3_src)
     (LOCAL: sim_local lc3_src lc1_tgt):
     sim_update
-      (State.mk rs [Stmt.instr i2; Stmt.instr (Instr.update r1 l1 rmw1 or1 ow1)]) lc1_src sc_k_src mem_k_src
-      (State.mk (RegFun.add r1 vret1 rs) [Stmt.instr i2]) lc1_tgt sc_k_tgt mem_k_tgt
+      (State.mk rs [Stmt.instr i2; Stmt.instr (Instr.update r1 l1 rmw1 or1 ow1)]) lc1_src sc0_src mem0_src
+      (State.mk (RegFun.add r1 vret1 rs) [Stmt.instr i2]) lc1_tgt sc0_tgt mem0_tgt
 .
 
 Lemma sim_update_step
-      st1_src lc1_src sc_k_src mem_k_src
-      st1_tgt lc1_tgt sc_k_tgt mem_k_tgt
-      (SIM: sim_update st1_src lc1_src sc_k_src mem_k_src
-                      st1_tgt lc1_tgt sc_k_tgt mem_k_tgt):
+      st1_src lc1_src sc0_src mem0_src
+      st1_tgt lc1_tgt sc0_tgt mem0_tgt
+      (SIM: sim_update st1_src lc1_src sc0_src mem0_src
+                      st1_tgt lc1_tgt sc0_tgt mem0_tgt):
   forall mem1_src mem1_tgt
     (MEMORY: sim_memory mem1_src mem1_tgt)
-    (FUTURE_SRC: Memory.future mem_k_src mem1_src)
-    (FUTURE_TGT: Memory.future mem_k_tgt mem1_tgt)
+    (FUTURE_SRC: Memory.future mem0_src mem1_src)
+    (FUTURE_TGT: Memory.future mem0_tgt mem1_tgt)
     (WF_SRC: Local.wf lc1_src mem1_src)
     (WF_TGT: Local.wf lc1_tgt mem1_tgt)
     (MEM_SRC: Memory.closed mem1_src)
